Basic definitions, statement formalized

FRACTRAN/Test.lean
@@ -1,3 +1,41 @@
+import Std.Data.Rat
 import Mathlib.Data.LazyList
 
-#check LazyList.singleton
+def FRACTRANprog : Type := List Rat
+
+def FRACTRANrun : Type := Int → Nat → Int
+
+def FRACTRANrun' : Type := Int -> LazyList Int
+
+def next' (prog : FRACTRANprog) (n : Int) : Option Int :=
+  match prog with
+  | []      => none
+  | q :: qs => if Rat.isInt (q * n)
+               then Rat.floor $ q * n -- coercion
+               else next' qs n
+
+def next (prog : FRACTRANprog) (n : Int) : Int :=
+  match prog with
+  | []      => 0
+  | q :: qs => if Rat.isInt (q * n)
+               then Rat.floor $ q * n
+               else next qs n
+
+unsafe def runProg' (prog : FRACTRANprog) : FRACTRANrun' :=
+  fun z ↦ match (next' prog z) with
+          | none   => LazyList.nil
+          | some k => LazyList.cons k $ runProg' prog k -- coercion
+
+def runProg (prog : FRACTRANprog) : FRACTRANrun :=
+  fun z n ↦ match n with
+  | Nat.zero => z
+  | Nat.succ k => next prog $ runProg prog z k
+
+def n : Int := 6
+#eval LazyList.toList $ runProg' [Rat.mk' 2 3] n
+#eval runProg [Rat.mk' 2 3] n 0
+
+def adder (a b : Nat) := runProg [Rat.mk' 2 3] (2^a * 3^b)
+
+theorem adder_adds : ∀ a b : Nat, ∃ K : Nat, (adder a b K = 2^(a + b) ∧ ∀ n : Nat, n > N → adder a b n = 0) := by
+  sorry
